Simpler partialsubst, keep only one proof of nam2mix_canonical

AltSubst.v
@@ -4,7 +4,7 @@
 (** The NatDed development, Pierre Letouzey, 2019.
     This file is released under the CC0 License, see the LICENSE file *)
 
-Require Import Defs NameProofs Nam Alpha Equiv.
+Require Import Defs NameProofs Nam Alpha Equiv Meta.
 Import ListNotations.
 Import Nam.Form.
 Local Open Scope bool_scope.
@@ -13,15 +13,15 @@ Local Open Scope eqb_scope.
 
 Module Subst.
 
-Definition t := substitution.
+Definition t := list (variable * term).
 
-Definition invars (sub : substitution) :=
+Definition invars (sub : t) :=
   List.fold_right (fun p vs => Names.add (fst p) vs) Names.empty sub.
 
-Definition outvars (sub : substitution) :=
+Definition outvars (sub : t) :=
   Names.unionmap (fun '(_,t) => Term.vars t) sub.
 
-Definition vars (sub : substitution) :=
+Definition vars (sub : t) :=
   Names.union (invars sub) (outvars sub).
 
 End Subst.
@@ -30,7 +30,7 @@ Module Alt.
 
 (** Term substitution *)
 
-Fixpoint term_substs (sub:substitution) t :=
+Fixpoint term_substs (sub:Subst.t) t :=
   match t with
   | Var v => list_assoc_dft v sub t
   | Fun f args => Fun f (List.map (term_substs sub) args)
@@ -41,7 +41,7 @@ Definition term_subst x u t := term_substs [(x,u)] t.
 (** Simultaneous substitution of many variables in a term.
     Capture of bounded variables is correctly handled. *)
 
-Fixpoint substs (sub : substitution) f :=
+Fixpoint substs (sub : Subst.t) f :=
  match f with
   | True | False => f
   | Pred p args => Pred p (List.map (term_substs sub) args)
@@ -93,3 +93,903 @@ Definition αeq f1 f2 := αeq_gen [] f1 [] f2.
 Definition AlphaEq f1 f2 := αeq f1 f2 = true.
 
 End Alt.
+
+
+Lemma invars_in sub v :
+  Names.In v (Subst.invars sub) <-> In v (map fst sub).
+Proof.
+ induction sub as [|(x,t) sub IH]; simpl. namedec.
+ nameiff. intuition.
+Qed.
+
+Lemma invars_app h h' :
+  Names.Equal (Subst.invars (h++h'))
+             (Names.union (Subst.invars h) (Subst.invars h')).
+Proof.
+ induction h; simpl; auto with set.
+Qed.
+
+Lemma invars_unassoc v h :
+  Names.Equal (Subst.invars (list_unassoc v h))
+             (Names.remove v (Subst.invars h)).
+Proof.
+ induction h as [|(x,u) h IH]; simpl.
+ - namedec.
+ - case eqbspec; simpl.
+   + intros ->. rewrite IH. namedec.
+   + intros NE. rewrite IH. namedec.
+Qed.
+
+Lemma outvars_app h h' :
+ Names.Equal (Subst.outvars (h++h'))
+            (Names.union (Subst.outvars h) (Subst.outvars h')).
+Proof.
+ unfold Subst.outvars.
+ apply unionmap_app.
+Qed.
+
+Lemma outvars_unassoc v h :
+ Names.Subset (Subst.outvars (list_unassoc v h))
+             (Subst.outvars h).
+Proof.
+ induction h as [|(x,t) h IH]; simpl.
+ - namedec.
+ - case eqbspec; simpl; namedec.
+Qed.
+
+(** Free variables after [substs] *)
+
+Lemma term_substs_vars h t :
+ Names.Subset (Term.vars (Alt.term_substs h t))
+             (Names.union (Names.diff (Term.vars t) (Subst.invars h))
+                         (Subst.outvars h)).
+Proof.
+ revert t.
+ fix IH 1. destruct t as [v|f l]; cbn.
+ - rewrite list_assoc_dft_alt.
+   assert (H := list_assoc_in2 h v).
+   assert (H' := list_assoc_notin h v).
+   destruct (list_assoc v h).
+   + specialize (H t).
+     unfold Subst.outvars.
+     intros y Hy.
+     rewrite Names.union_spec, unionmap_in.
+     right. exists (v,t); auto.
+   + simpl. intros y. rewrite Names.singleton_spec. intros ->.
+     nameiff. left; split; auto.
+     rewrite invars_in; intuition.
+ - clear f. revert l.
+   fix IH' 1. destruct l as [|t l]; cbn -[Names.diff].
+   + namedec.
+   + specialize (IH t). specialize (IH' l). namedec.
+Qed.
+
+Lemma substs_freevars h f :
+ Names.Subset (freevars (Alt.substs h f))
+             (Names.union (Names.diff (freevars f) (Subst.invars h))
+                         (Subst.outvars h)).
+Proof.
+ revert h.
+ induction f; cbn -[Subst.invars Subst.outvars Names.diff]; intros; auto.
+ - namedec.
+ - namedec.
+ - apply (term_substs_vars h (Fun "" l)).
+ - rewrite IHf1, IHf2. namedec.
+ - destruct (Names.mem _ _) eqn:E; simpl.
+   + setfresh vars z Hz.
+     rewrite IHf; simpl.
+     rewrite invars_unassoc, outvars_unassoc. namedec.
+   + rewrite IHf; simpl.
+     rewrite invars_unassoc, outvars_unassoc. namedec.
+Qed.
+
+(** [Term.substs] may do nothing *)
+
+Lemma term_substs_notin h t :
+ Names.Empty (Names.inter (Term.vars t) (Subst.invars h)) ->
+ Alt.term_substs h t = t.
+Proof.
+ induction t as [v |f l IH] using term_ind'; intros EM; cbn in *.
+ - rewrite list_assoc_dft_alt.
+   assert (NI : ~In v (map fst h)).
+   { rewrite <- invars_in. namedec. }
+   rewrite <- list_assoc_notin in NI. now rewrite NI.
+ - f_equal. clear f.
+   apply map_id_iff.
+   intros a Ha. apply IH; auto. intros v. nameiff. intros (Hv,Hv').
+   apply (EM v). nameiff. split; auto.
+   rewrite unionmap_in. now exists a.
+Qed.
+
+
+(** Let's show that [Alt.substs] produce alpha-equivalent results.
+    This is surprinsingly painful to prove, we'll need quite
+    some tooling first.
+*)
+
+Definition renaming := list (variable*variable).
+
+Definition putVar : variable*variable -> variable*term :=
+ fun '(a,b) => (a,Var b).
+
+Definition chgVar : renaming -> variable -> variable :=
+  fun h v => list_assoc_dft v h v.
+
+Lemma fst_putVar (h:renaming) :
+  map fst (map putVar h) = map fst h.
+Proof.
+ induction h as [|(a,b) l IH]; simpl; f_equal; auto.
+Qed.
+
+Lemma assoc_putVar (h:renaming) v :
+  list_assoc v (map putVar h) = option_map Var (list_assoc v h).
+Proof.
+ induction h as [|(a,b) h IH]; simpl; auto.
+ case eqbspec; auto.
+Qed.
+
+Lemma unassoc_putVar (h:renaming) v :
+  list_unassoc v (map putVar h) = map putVar (list_unassoc v h).
+Proof.
+ induction h as [|(a,b) h IH]; simpl; auto.
+ case eqbspec; simpl; intros; f_equal; auto.
+Qed.
+
+Lemma chgVar_some (h:renaming) x z :
+ list_assoc x h = Some z -> chgVar h x = z.
+Proof.
+ unfold chgVar. rewrite list_assoc_dft_alt. now intros ->.
+Qed.
+
+Lemma chgVar_none (h:renaming) x :
+ list_assoc x h = None -> chgVar h x = x.
+Proof.
+ unfold chgVar. rewrite list_assoc_dft_alt. now intros ->.
+Qed.
+
+Lemma chgVar_unassoc_at x (h:renaming) :
+  chgVar (list_unassoc x h) x = x.
+Proof.
+  unfold chgVar.
+  induction h as [|(a,b) h IH]; simpl in *; auto.
+  repeat (case eqbspec; simpl; auto). congruence.
+Qed.
+
+Lemma chgVar_unassoc_else x y (h:renaming) :
+  x<>y -> chgVar (list_unassoc x h) y = chgVar h y.
+Proof.
+  unfold chgVar.
+  induction h as [|(a,b) h IH]; simpl in *; auto.
+  repeat (case eqbspec; simpl; auto). congruence.
+Qed.
+
+Fixpoint Inv vs (h:renaming) :=
+  match h with
+  | [] => Logic.True
+  | (v,z)::h => ~Names.In z vs /\
+                (forall a b, In (a,b) h -> z<>a/\z<>b) /\
+                Inv vs h
+  end.
+
+Lemma Inv_subset vs vs' h :
+  Names.Subset vs vs' -> Inv vs' h -> Inv vs h.
+Proof.
+ induction h as [|(v,z) h IH]; simpl; intuition.
+Qed.
+
+Lemma Inv_add vs x (h:renaming) :
+  Names.Subset vs (Names.add x vs) ->
+  ~Names.In x (Subst.vars (map putVar h)) ->
+  Inv vs h -> Inv (Names.add x vs) h.
+Proof.
+ induction h as [|(v,z) h IH]; simpl; auto.
+ intros SU NI (NI' & H & IV).
+ unfold Subst.vars in *. simpl in NI.
+ split; [|split; auto with set].
+ nameiff.
+ intros [->|IN]; auto with set.
+Qed.
+
+Lemma Inv_notin vs (h:renaming) v z :
+  Inv vs h -> list_assoc v h = Some z -> ~Names.In z vs.
+Proof.
+ induction h as [|(a,b) h IH]; simpl; try easy.
+ intros (H & H' & IV).
+ case eqbspec; auto.
+ now intros <- [= ->].
+Qed.
+
+Lemma Inv_notin_unassoc vs (h:renaming) v z :
+ Inv vs h -> list_assoc v h = Some z ->
+ ~Names.In z (Subst.outvars (map putVar (list_unassoc v h))).
+Proof.
+ induction h as [|(a,b) h IH]; simpl; try easy.
+ intros (H & H' & IV).
+ rewrite eqb_sym.
+ case eqbspec; simpl.
+ - intros -> [= ->].
+   rewrite <- unassoc_putVar.
+   unfold Subst.outvars.
+   rewrite unionmap_in.
+   intros ((x,t) & IN & IN').
+   rewrite unassoc_in, in_map_iff in IN'.
+   destruct IN' as (((a,b) & [=] & IN'),NE).
+   subst t a. cbn in *. apply H' in IN'. namedec.
+ - intros NE EQ.
+   specialize (IH IV EQ). unfold Subst.vars in IH.
+   assert (IN: In (v,z) h).
+   { now apply list_assoc_in2. }
+   apply H' in IN.
+   namedec.
+Qed.
+
+Lemma Inv_notin' vs (h:renaming) (v x:variable) :
+  Inv vs h -> (Names.In x vs \/ list_assoc v h = Some x) ->
+  ~Names.In x (Subst.outvars (map putVar (list_unassoc v h))).
+Proof.
+ intros IV.
+ induction h as [|(a,b) h IH]; simpl in *; auto.
+ - namedec.
+ - destruct IV as (H & H' & IV).
+   rewrite eqb_sym.
+   case eqbspec; simpl.
+   + intros -> [IN|[= ->]]. intuition.
+     unfold Subst.outvars. rewrite unionmap_map_in.
+     intros ((a,b) & IN & IN'). rewrite unassoc_in in IN'.
+     simpl in IN. rewrite Names.singleton_spec in IN.
+     destruct (H' a b); intuition.
+   + intros NE [IN|SO];
+      rewrite Names.union_spec, Names.singleton_spec.
+     * intuition.
+     * intros [<-|IN]; [|intuition].
+       apply list_assoc_in2 in SO. now apply H' in SO.
+Qed.
+
+Lemma Inv_inj vs (h:renaming) x y z :
+ Inv vs h ->
+ list_assoc x h = Some z ->
+ list_assoc y h = Some z ->
+ x = y.
+Proof.
+ induction h as [|(a,b) h IH]; cbn; try easy.
+ intros (H & H' & IV).
+ repeat case eqbspec; auto.
+ - congruence.
+ - intros NE <- [= <-] EQ.
+   apply list_assoc_in2 in EQ. now apply H' in EQ.
+ - intros <- NE [= <-] EQ.
+   symmetry in EQ. apply list_assoc_in2 in EQ. now apply H' in EQ.
+Qed.
+
+Lemma Inv_inj' vs (h:renaming) (x y:variable) :
+  Inv vs h ->
+  Names.In x vs -> Names.In y vs ->
+  chgVar h x = chgVar h y -> x = y.
+Proof.
+ intros IV Hx Hy.
+ unfold chgVar. rewrite !list_assoc_dft_alt.
+ destruct (list_assoc x h) eqn:E, (list_assoc y h) eqn:E'.
+ - intros <-. eapply Inv_inj; eauto.
+ - intros ->. eapply Inv_notin in E; eauto. easy.
+ - intros ->. eapply Inv_notin in E'; eauto. easy.
+ - easy.
+Qed.
+
+Lemma Inv_unassoc vs (h:renaming) v :
+ Inv vs h -> Inv vs (list_unassoc v h).
+Proof.
+ induction h as [|(a,b) h IH]; simpl; auto.
+ intros (H & H' & IV).
+ case eqbspec; simpl; auto.
+ intros NE. do 2 (split; auto).
+ intros a' b'. rewrite unassoc_in. firstorder.
+Qed.
+
+Lemma nam2mix_substs_rename_aux stk stk' v (h:renaming) f :
+  let g := list_unassoc v h in
+  In (chgVar h v) stk \/ ~Names.In (chgVar h v) (freevars f) ->
+  In v stk ->
+  nam2mix (stk ++ map (chgVar h) stk') f =
+  nam2mix (stk ++ map (chgVar g) stk') f.
+Proof.
+ revert stk.
+ induction stk' as [|x stk' IH]; simpl; intros stk OR IN; auto.
+ case (eqbspec x v).
+ - intros ->.
+   rewrite chgVar_unassoc_at.
+   rewrite nam2mix_shadowstack' with (y:=v) by intuition.
+   rewrite cons_app, <- app_ass, IH, app_ass; simpl; auto.
+   rewrite in_app_iff; intuition.
+   rewrite in_app_iff; right; simpl; auto.
+ - intros NE.
+   rewrite chgVar_unassoc_else by auto.
+   rewrite cons_app, <- app_ass, IH, app_ass; simpl; auto.
+   rewrite in_app_iff; intuition.
+   rewrite in_app_iff; intuition.
+Qed.
+
+Lemma nam2mix_term_chgVar_some stk (h:renaming) (v z:variable) :
+  Inv (Names.union (Names.of_list stk) (Names.singleton v)) h ->
+  list_assoc v h = Some z -> In v stk ->
+  nam2mix_term (map (chgVar h) stk) (Var z) =
+  nam2mix_term stk (Var v).
+Proof.
+ intros IV EQ IN. simpl.
+ induction stk; simpl in *; try easy.
+ case (eqbspec v a).
+ - intros <-. now rewrite (chgVar_some h v z), eqb_refl.
+ - intros NE.
+   case eqbspec.
+   + intros EQ'. destruct NE.
+     rewrite <- (chgVar_some _ _ _ EQ) in EQ'.
+     eapply Inv_inj'; eauto with set.
+   + intros NE'.
+     destruct IN; [subst;easy|].
+     assert (H' : Inv (Names.union (Names.of_list stk) (Names.singleton v)) h).
+     { eapply Inv_subset; eauto. namedec. }
+     specialize (IHstk H' H).
+     destruct (list_index z (map (chgVar h) stk)),
+              (list_index v stk); simpl; try easy.
+     injection IHstk as ->; auto.
+Qed.
+
+Lemma nam2mix_term_chgVar_none stk (h:renaming) (v:variable) :
+  Inv (Names.union (Names.of_list stk) (Names.singleton v)) h ->
+  list_assoc v h = None ->
+  nam2mix_term (map (chgVar h) stk) (Var v) =
+  nam2mix_term stk (Var v).
+Proof.
+ intros IV EQ. simpl.
+ induction stk; simpl in *; auto.
+ case (eqbspec v a).
+ - intros <-. now rewrite chgVar_none, eqb_refl.
+ - intros NE.
+   case eqbspec.
+   + intros EQ'. destruct NE.
+     rewrite <- (chgVar_none _ _ EQ) in EQ'.
+     eapply Inv_inj'; eauto with set.
+   + intros NE'.
+     assert (H : Inv (Names.union (Names.of_list stk) (Names.singleton v)) h).
+     { eapply Inv_subset; eauto. namedec. }
+     specialize (IHstk H).
+     destruct (list_index v (map (chgVar h) stk)),
+              (list_index v stk); simpl; try easy.
+     injection IHstk as ->; auto.
+Qed.
+
+Lemma nam2mix_term_substs_rename stk (h:renaming) t :
+ Inv (Names.union (Names.of_list stk) (Term.vars t)) h ->
+ (forall a b, In (a,b) h -> In a stk) ->
+ nam2mix_term (map (chgVar h) stk) (Alt.term_substs (map putVar h) t) =
+ nam2mix_term stk t.
+Proof.
+ revert t.
+ fix IH 1. destruct t as [v|f l]; cbn; intros IV SU.
+ - clear IH. rewrite list_assoc_dft_alt.
+   rewrite assoc_putVar.
+   destruct (list_assoc v h) as [z|] eqn:E; simpl.
+   + apply nam2mix_term_chgVar_some; auto.
+     apply list_assoc_in2 in E. eapply SU; eauto.
+   + apply nam2mix_term_chgVar_none; auto.
+ - f_equal. clear f.
+   revert l IV.
+   fix IH' 1. destruct l as [|t l]; cbn; intros IV; auto.
+   f_equal.
+   apply IH; auto. eapply Inv_subset; eauto. namedec.
+   apply IH'; auto. eapply Inv_subset; eauto. namedec.
+Qed.
+
+Lemma nam2mix_substs_rename stk (h:renaming) f:
+ Inv (Names.union (Names.of_list stk) (allvars f)) h ->
+ (forall a b, In (a,b) h -> In a stk) ->
+ nam2mix (map (chgVar h) stk) (Alt.substs (map putVar h) f) =
+ nam2mix stk f.
+Proof.
+ revert stk h.
+ induction f; intros stk h IV SU; cbn in *; auto.
+ - f_equal.
+   injection (nam2mix_term_substs_rename stk h (Fun "" l)); auto.
+ - f_equal; auto.
+ - f_equal. apply IHf1; auto. eapply Inv_subset; eauto. namedec.
+   apply IHf2; auto. eapply Inv_subset; eauto. namedec.
+ - set (g' := list_unassoc v (map putVar h)).
+   set (g := list_unassoc v h).
+   assert (~Names.In v (Subst.outvars g')).
+   { unfold g'. rewrite unassoc_putVar.
+     eapply Inv_notin'; eauto. left; namedec. }
+   rewrite mem_false by trivial; simpl.
+   f_equal.
+   rewrite <- IHf with (h:=g).
+   2:{ apply Inv_unassoc.
+       eapply Inv_subset; eauto. simpl; namedec. }
+   2:{ intros a b. unfold g.
+       rewrite unassoc_in. intros (IN,_); simpl; eauto. }
+   cbn.
+   rewrite chgVar_none.
+   2:{ apply list_assoc_notin.
+       (* sous-lemme ? *)
+       unfold g. rewrite in_map_iff.
+       intros ((a,b) & <- & IN); simpl in IN.
+       rewrite unassoc_in in IN. easy. }
+   unfold g at 2. rewrite <- unassoc_putVar. fold g'.
+   apply (nam2mix_substs_rename_aux [v]); simpl; auto.
+   rewrite substs_freevars, freevars_allvars.
+   destruct (list_assoc v h) as [z|] eqn:Hz.
+   + right.
+     rewrite (chgVar_some _ _ _ Hz).
+     assert (IV2 := Inv_notin _ _ _ _ IV Hz).
+     assert (IV3 := Inv_notin' _ _ _ _ IV (or_intror _ Hz)).
+     rewrite <- unassoc_putVar in IV3. fold g' in IV3.
+     namedec.
+   + left; left. symmetry. now apply chgVar_none.
+Qed.
+
+Lemma nam2mix_term_substs stk h x u t:
+ Inv (Names.unions [Names.of_list stk;
+                   Term.vars t;
+                   Names.add x (Term.vars u)]) h ->
+ (forall a b , In (a,b) h -> In a stk) ->
+ ~In x stk ->
+ (forall v, In v stk -> ~Names.In (chgVar h v) (Term.vars u)) ->
+ nam2mix_term (map (chgVar h) stk)
+              (Alt.term_substs (map putVar h ++ [(x,u)]) t) =
+ Mix.fsubst x (nam2mix_term [] u) (nam2mix_term stk t).
+Proof.
+ intros IV SU NI CL.
+ revert t IV.
+ fix IH 1. destruct t as [v|f l]; cbn; intros IV.
+ - clear IH. rewrite list_assoc_dft_alt.
+   destruct (In_dec string_dec v (map fst h)) as [IN|NI'].
+   + assert (In v (map fst (map putVar h))).
+     { rewrite map_map. rewrite in_map_iff in *.
+       destruct IN as ((a,b) & EQ & IN). now exists (a,b). }
+     rewrite list_assoc_app_l by auto.
+     rewrite assoc_putVar.
+     rewrite <- list_assoc_in in IN.
+     destruct (list_assoc v h) as [z|] eqn:E; simpl; try easy.
+     assert (IN' : In v stk).
+     { now apply list_assoc_in2, SU in E. }
+     generalize (nam2mix_term_chgVar_some stk h v z).
+     simpl.
+     intros ->; auto; [ | eapply Inv_subset; eauto; namedec].
+     rewrite <- list_index_in in IN'.
+     now destruct (list_index v stk).
+   + assert (~In v (map fst (map putVar h))).
+     { rewrite map_map. rewrite in_map_iff in *.
+       intros ((a,b) & EQ & IN). apply NI'. now exists (a,b). }
+     rewrite list_assoc_app_r by auto.
+     simpl. case eqbspec; simpl.
+     * intros <-. apply list_index_notin in NI.
+       change Names.elt with variable in *.
+       rewrite NI. cbn. unfold Mix.varsubst. rewrite eqb_refl.
+       apply nam2mix_term_nostack.
+       intros y. rewrite in_map_iff. intros (x & <- & Hx); auto.
+     * intros NE.
+       generalize (nam2mix_term_chgVar_none stk h v).
+       simpl.
+       intros ->; auto.
+       2:{ eapply Inv_subset; eauto. namedec. }
+       2:{ now apply list_assoc_notin. }
+       unfold Mix.fsubst.
+       rewrite term_vmap_id; auto.
+       intros y. unfold Mix.varsubst.
+       destruct (list_index v stk); cbn; nameiff; intuition.
+ - f_equal. clear f.
+   revert l IV.
+   fix IH' 1. destruct l as [|t l]; cbn; intros IV; auto.
+   f_equal.
+   apply IH; auto. eapply Inv_subset; eauto. simpl. namedec.
+   apply IH'; auto. eapply Inv_subset; eauto. simpl. namedec.
+Qed.
+
+Ltac namedec00 := clear; nameiff; intuition auto.
+
+Lemma stack_notin_term
+  (v z z' : variable)(t : term)
+  (stk : list variable)(h g : renaming) g' :
+  g = list_unassoc v h ->
+  g' = map putVar g ->
+  ~Names.In z (Term.vars t) ->
+  ~Names.In z' (Names.union (Subst.vars g') (Names.add v (Term.vars t))) ->
+  let stk' := map (fun a : variable => if a =? z then z' else a) stk in
+  (forall v : variable,
+    In v stk -> ~ Names.In (chgVar h v) (Term.vars t)) ->
+  forall v' : variable,
+    In v' (v :: stk') ->
+    ~ Names.In (chgVar ((v, z) :: g) v') (Term.vars t).
+Proof.
+ intros Hg Hg' Hz Hz' stk' CL v0 [<-|IN].
+ - unfold chgVar. simpl. rewrite eqb_refl. namedec0.
+ - unfold stk' in IN. rewrite in_map_iff in IN.
+   destruct IN as (y & EQ & IN). revert EQ.
+   case eqbspec.
+   + intros -> <-.
+     rewrite chgVar_none; [namedec0|]; simpl.
+     case eqbspec; [intros <-;namedec0|].
+     intros _.
+     assert (NO : list_assoc z' g' = None).
+     { apply list_assoc_notin.
+       rewrite <- invars_in. unfold Subst.vars in Hz'. namedec0. }
+     revert NO.
+     rewrite Hg'. rewrite assoc_putVar.
+     now destruct (list_assoc z' g).
+   + intros NE' ->. unfold chgVar. simpl.
+     case eqbspec; [namedec0|].
+     intros NE''.
+     fold (chgVar g v0). rewrite Hg.
+     rewrite chgVar_unassoc_else by auto.
+     now apply CL.
+Qed.
+
+Lemma nam2mix_shadowstack_map stk stk' x y f :
+ In x stk \/ ~Names.In x (freevars f) ->
+ In y stk \/ ~Names.In y (freevars f) ->
+ nam2mix (stk++map (fun a => if a =?x then y else a) stk') f =
+ nam2mix (stk++stk') f.
+Proof.
+ intros Hx Hy. apply nam2mix_indep.
+ intros v Hv.
+ destruct (in_dec string_dec v stk).
+ - rewrite 2 list_index_app_l; auto.
+ - rewrite 2 list_index_app_r; auto. f_equal.
+   induction stk' as [|a stk' IH]; auto.
+   simpl. rewrite IH.
+   case (eqbspec a x); auto.
+   repeat case eqbspec; intros; subst; intuition.
+Qed.
+
+Lemma Inv_Inv
+  (x v z z' : variable)(t : term)(f : formula)
+  (stk : list variable)(h g : renaming) g' :
+  let vars := Names.union (Names.add v (allvars f))
+                         (Names.add x (Term.vars t)) in
+  Inv (Names.union (Names.of_list stk) vars) h ->
+  g = list_unassoc v h ->
+  g' = map putVar g ->
+  ~Names.In z (Names.union (Subst.vars g') vars) ->
+  ~Names.In z' (Names.union (Subst.vars g') vars) ->
+  ~Names.In z' (Names.of_list stk) ->
+  let stk' := map (fun a : variable => if a =? z then z' else a) stk in
+  Inv
+    (Names.union (Names.of_list (v :: stk'))
+       (Names.union (allvars f)
+          (Names.union (Names.add x (Term.vars t)) Names.empty)))
+    ((v, z) :: g).
+Proof.
+ intros vars IV Hg Hg' Hz Hz' Hz'' stk'.
+ simpl. split; [|split].
+ - assert (NI' : ~Names.In z (Names.of_list stk')).
+   { rewrite names_of_list_in.
+     unfold stk'. rewrite in_map_iff.
+     intros (z0 & EQ & IN). rewrite <- names_of_list_in in IN.
+     revert EQ. case eqbspec; [|easy].
+     intros -> <-; exact (Hz'' IN). }
+   revert Hz NI'. unfold vars. namedec00.
+ - intros a b Hab.
+   assert (In (a,Var b) g').
+   { rewrite Hg'. rewrite in_map_iff. now exists (a,b). }
+   assert (Names.In a (Subst.invars g')).
+   { rewrite invars_in. rewrite in_map_iff. now exists (a,Var b). }
+   assert (Names.In b (Subst.outvars g')).
+   { unfold Subst.outvars. rewrite unionmap_in. exists (a,Var b).
+     simpl. auto with set. }
+   unfold vars, Subst.vars in Hz.
+   split; namedec.
+ - apply Inv_unassoc with (v:=v) in IV. rewrite <- Hg in IV.
+   apply Inv_add with (x:=z') in IV;
+     [ | namedec| rewrite <- Hg'; revert Hz'; namedec00].
+   eapply Inv_subset; eauto.
+   assert (Names.Subset (Names.of_list stk')
+                        (Names.add z' (Names.of_list stk))).
+   { unfold stk'. clear. intros x.
+     rewrite Names.add_spec, !names_of_list_in, in_map_iff.
+     intros (x0 & EQ & IN). revert EQ.
+     case eqbspec; intros; subst; auto. }
+   rewrite H. intro. unfold vars. namedec00.
+Qed.
+
+Lemma nam2mix_altsubsts_aux1
+  (x v z z' : variable)(t : term)(f : formula)
+  (stk : list variable)(h g : renaming) g' :
+  let vars := Names.union (Names.add v (allvars f))
+                         (Names.add x (Term.vars t)) in
+  Inv vars h ->
+  g = list_unassoc v h ->
+  g' = map putVar g ->
+  ~Names.In z (Names.union (Subst.vars g') vars) ->
+  ~Names.In z' (Names.union (Subst.vars g') vars) ->
+  ~Names.In z' (Names.of_list stk) ->
+  (In v stk -> chgVar h v <> v) ->
+  let stk' := map (fun a : variable => if a =? z then z' else a) stk in
+  nam2mix (z :: map (chgVar h) stk)
+    (Alt.substs ((v, Var z) :: g' ++ [(x, t)]) f) =
+  nam2mix (map (chgVar ((v, z) :: g)) (v :: stk'))
+    (Alt.substs (map putVar ((v, z) :: g) ++ [(x, t)]) f).
+Proof.
+ intros vars IV Hg Hg' Hz Hz' Hz'' CL stk'.
+ unfold Subst.vars in *; simpl in *.
+ rewrite chgVar_some with (z:=z) by (simpl; now rewrite eqb_refl).
+ rewrite <-Hg'.
+ set (f' := Alt.substs _ f).
+ unfold stk'. clear stk'. rewrite map_map.
+ apply nam2mix_indep.
+ intros y Hy.
+ simpl.
+ case eqbspec; auto.
+ intros Hyz. f_equal.
+ unfold f' in Hy.
+ rewrite substs_freevars in Hy. simpl in Hy.
+ rewrite invars_app, outvars_app in Hy.
+ simpl in Hy.
+ rewrite freevars_allvars in Hy.
+ assert (Hyz' : y <> z').
+ { intros ->. revert Hz' Hy Hyz. unfold vars. namedec00. }
+ assert (H : ~Names.In z (Subst.invars g')) by namedec0.
+ assert (Hzv : z<>v) by (unfold vars in Hz; namedec0).
+ rewrite Hg',Hg, <- unassoc_putVar in H.
+ rewrite invars_unassoc in H.
+ assert (Hzh : ~Names.In z (Subst.invars (map putVar h))).
+ { revert H Hzv. namedec00. }
+ clear H.
+ rewrite invars_in, fst_putVar in Hzh.
+ assert (Hhz : chgVar h z = z).
+ { apply chgVar_none. now apply list_assoc_notin. }
+ assert (Hgz' : chgVar ((v, z) :: g) z' = z').
+ { apply chgVar_none. simpl.
+   case eqbspec; [unfold vars in Hz';namedec0|].
+   intros NE2. apply list_assoc_notin.
+   rewrite <- fst_putVar, <- Hg'.
+   rewrite <- invars_in. namedec0. }
+ assert (NI := Inv_notin _ _ v (chgVar h v) IV).
+ assert (NI' := Inv_notin_unassoc _ _ v (chgVar h v) IV).
+ clear IV.
+ revert stk CL Hz''.
+ induction stk as [|s stk IH]; simpl; auto.
+ intros CL Hz''.
+ rewrite Names.add_spec in Hz''.
+ apply Decidable.not_or in Hz''.
+ destruct Hz'' as (Hsz',Hz'').
+ case (eqbspec s z).
+ - intros ->.
+   rewrite Hhz, Hgz'.
+   do 2 (case eqbspec; easy || intros _). f_equal; auto.
+ - intros Hsz.
+   case (eqbspec s v).
+   + intros ->.
+     set (hv := chgVar h v) in *.
+     unfold chgVar at 2. simpl. rewrite eqb_refl.
+     case (eqbspec y z); easy || intros _.
+     case eqbspec; [|intros;f_equal;auto].
+     intros ->. exfalso.
+     clear IH Hz' Hyz' Hgz'.
+     assert (list_assoc v h = Some hv).
+     { generalize (CL (or_introl _ (eq_refl))).
+       unfold hv, chgVar. rewrite list_assoc_dft_alt.
+       destruct list_assoc; intuition. }
+     generalize (NI H) (NI' H) Hy Hyz.
+     rewrite <- Hg, <- Hg'. unfold vars. namedec00.
+   + intros NE.
+     replace (chgVar ((v, z)::g) s) with (chgVar h s).
+     { case eqbspec; intros; f_equal; auto. }
+     { symmetry. unfold chgVar at 1. simpl.
+       case eqbspec; easy || intros _.
+       fold (chgVar g s). rewrite Hg.
+       apply chgVar_unassoc_else; auto. }
+Qed.
+
+Lemma form_altsubsts_aux2
+  (x v : variable)(t : term)(f : formula)
+  (stk : list variable)(h g : renaming) g' :
+  let vars := Names.union (Names.add v (allvars f))
+                         (Names.add x (Term.vars t)) in
+  Inv vars h ->
+  g = list_unassoc v h ->
+  g' = map putVar g ->
+  let f' := Alt.substs (g' ++ [(x,t)]) f in
+  nam2mix (v :: map (chgVar h) stk) f' =
+  nam2mix (map (chgVar g) (v::stk)) f'.
+Proof.
+ intros vars IV Hg Hg' f'.
+ simpl.
+ rewrite Hg at 1. rewrite chgVar_unassoc_at.
+ apply nam2mix_indep.
+ intros y Hy.
+ simpl. case eqbspec; auto.
+ intros NE. f_equal.
+ assert (NE' : y <> chgVar h v).
+ { unfold chgVar. rewrite list_assoc_dft_alt.
+   destruct (list_assoc v h) eqn:E; auto.
+   intros <-.
+   revert Hy.
+   unfold f'.
+   rewrite substs_freevars, freevars_allvars.
+   rewrite invars_app, outvars_app.
+   generalize (Inv_notin _ _ _ _ IV E). simpl.
+   generalize (Inv_notin_unassoc _ _ _ _ IV E).
+   rewrite <- Hg, <- Hg'.
+   revert NE. unfold vars. namedec00. }
+ rewrite Hg.
+ clear - NE NE'.
+ induction stk; simpl; auto.
+ case (eqbspec a v).
+ - intros ->.
+   rewrite chgVar_unassoc_at.
+   do 2 (case eqbspec; easy || intros _).
+   now f_equal.
+ - intros NE2.
+   rewrite chgVar_unassoc_else; auto.
+   case eqbspec; auto. intros _. now f_equal.
+Qed.
+
+Lemma nam2mix_altsubsts (stk:list variable) h (x:variable) t f:
+ Inv (Names.unions [Names.of_list stk;
+                   allvars f;
+                   Names.add x (Term.vars t)]) h ->
+ (forall a b , In (a,b) h -> In a stk) ->
+ ~In x stk ->
+ (forall v, In v stk -> ~Names.In (chgVar h v) (Term.vars t)) ->
+ nam2mix (map (chgVar h) stk)
+         (Alt.substs (map putVar h ++ [(x,t)]) f) =
+ Mix.fsubst x (nam2mix_term [] t) (nam2mix stk f).
+Proof.
+ revert stk h.
+ induction f; intros stk h IV SU NI CL; cbn in *; auto.
+ - f_equal.
+   injection (nam2mix_term_substs stk h x t (Fun "" l)); auto.
+ - f_equal; auto.
+ - f_equal. apply IHf1; auto. eapply Inv_subset; eauto. namedec.
+   apply IHf2; auto. eapply Inv_subset; eauto. namedec.
+ - rewrite !unassoc_app. cbn.
+   set (g' := list_unassoc v (map putVar h)).
+   set (g := list_unassoc v h).
+   assert (Hg : g' = map putVar g).
+   { unfold g', g. apply unassoc_putVar. }
+   case eqbspec; cbn.
+   + (* x = v *)
+     intros <-.
+     rewrite app_nil_r.
+     unfold Mix.fsubst.
+     rewrite form_vmap_id.
+     2:{ intros v. unfold Mix.varsubst. case eqbspec; auto.
+         intros <-. rewrite nam2mix_fvars. simpl. namedec. }
+     change
+       (nam2mix (map (chgVar h) stk)
+                (Alt.substs (map putVar h) (Quant q x f))
+        = nam2mix stk (Quant q x f)).
+     apply nam2mix_substs_rename; auto.
+     eapply Inv_subset; eauto. cbn. namedec.
+   + (* x <> v *)
+     intros NE.
+     destruct (Names.mem _ _) eqn:MM; cbn; f_equal;
+     rewrite outvars_app in MM; simpl in MM.
+     * (* Capture of variable v, which occurs in t *)
+       assert (IN : Names.In v (Term.vars t)).
+       { revert MM.
+         rewrite Names.mem_spec.
+         rewrite Hg. unfold g.
+         generalize (Inv_notin' _ _ v v IV). namedec00. }
+       clear MM.
+       setfresh vars z Hz.
+       destruct (exist_fresh (Names.union vars (Names.of_list stk)))
+        as (z',Hz').
+       set (stk' := map (fun a => if a =? z then z' else a) stk).
+       rewrite Names.union_spec in Hz'. apply Decidable.not_or in Hz'.
+       destruct Hz' as (Hz',Hz'2).
+       unfold vars in Hz,Hz'. clear vars.
+       rewrite outvars_app, invars_app in Hz,Hz'.
+       simpl in Hz, Hz'.
+       assert (CL' : In v stk -> chgVar h v <> v).
+       { intros IN' EQ. apply (CL v IN'). now rewrite EQ. }
+       erewrite nam2mix_altsubsts_aux1; eauto; fold stk'; fold g.
+       2:{clear -IV. eapply Inv_subset; eauto. simpl. intro. namedec00. }
+       2:{revert Hz. unfold Subst.vars; simpl. namedec00. }
+       2:{revert Hz'. unfold Subst.vars; simpl. namedec00. }
+       rewrite IHf; clear IHf.
+       { f_equal.
+         apply (nam2mix_shadowstack_map [v] stk);
+          right; rewrite freevars_allvars; namedec0. }
+       { eapply Inv_Inv with (h:=h); auto.
+         eapply Inv_subset; eauto. intro. namedec00.
+         revert Hz. rewrite <- Hg. unfold Subst.vars. namedec00.
+         revert Hz'. rewrite <- Hg. unfold Subst.vars. namedec00. }
+       { clear CL CL' IN.
+         intros a b [[= -> ->]|IN]; simpl; auto.
+         assert (Names.In a (Subst.invars g')).
+         { unfold g'.
+           rewrite invars_in. rewrite unassoc_putVar. fold g.
+           rewrite map_map. apply in_map_iff. now exists (a,b). }
+         assert (a <> z) by (intros ->; namedec0).
+         unfold g in IN. rewrite unassoc_in in IN. right.
+         unfold stk'. rewrite in_map_iff. exists a.
+         case eqbspec; try easy. split; auto. eapply SU. apply IN. }
+       { clear CL CL' IN.
+         intros [->|IN]; [easy|]. unfold stk' in IN. rewrite in_map_iff in IN.
+         destruct IN as (x0 & EQ & IN). revert EQ.
+         case eqbspec; intros; subst; auto. namedec0. }
+       { apply stack_notin_term with (h:=h)(g':=g'); auto.
+         revert Hz. namedec00.
+         revert Hz'. unfold Subst.vars. namedec00. }
+     * (* No capture of variable v *)
+       assert (~Names.In v (Term.vars t)).
+       { simpl in MM. rewrite <-not_true_iff_false, Names.mem_spec in MM.
+         namedec0. }
+       clear MM.
+       rewrite form_altsubsts_aux2 with (g:=g); auto.
+       2:{clear -IV. eapply Inv_subset; eauto. simpl. intro. namedec00. }
+       rewrite Hg.
+       apply IHf; clear IHf.
+       { apply Inv_unassoc.
+         eapply Inv_subset; eauto. simpl. namedec. }
+       { intros a b. unfold g.
+         rewrite unassoc_in. intros (IN,_); simpl; eauto. }
+       { simpl. intros [->|IN]; intuition. }
+       { intros y.
+         case (eqbspec y v).
+         - intros -> _. unfold g. now rewrite chgVar_unassoc_at.
+         - intros NE' [->|IN]; [easy|].
+           unfold g. rewrite chgVar_unassoc_else; auto. }
+Qed.
+
+(** And at last : *)
+
+Lemma nam2mix_altsubst x t f:
+ nam2mix [] (Alt.subst x t f) = nam2mix [] (subst x t f).
+Proof.
+ rewrite nam2mix0_subst_fsubst.
+ apply (nam2mix_altsubsts [] []); simpl; intuition.
+Qed.
+
+Lemma subst_alt x t f:
+ AlphaEq (Alt.subst x t f) (subst x t f).
+Proof.
+ apply nam2mix_canonical.
+ apply nam2mix_altsubst.
+Qed.
+
+Instance : Proper (eq ==> eq ==> AlphaEq ==> AlphaEq) Alt.subst.
+Proof.
+ intros x x' <- t t' <- f f' Hf.
+ now rewrite !subst_alt, Hf.
+Qed.
+
+Lemma altsubst_altsubst x y u v f :
+ x<>y -> ~Names.In x (Term.vars v) ->
+ AlphaEq (Alt.subst y v (Alt.subst x u f))
+         (Alt.subst x (Term.subst y v u) (Alt.subst y v f)).
+Proof.
+ intros.
+ rewrite !subst_alt.
+ apply subst_subst; auto.
+Qed.
+
+Lemma altsubst_QuGen (x z:variable) t q v f :
+ x<>v ->
+ ~Names.In z (Names.add x (Names.union (freevars f) (Term.vars t))) ->
+ AlphaEq (Alt.subst x t (Quant q v f))
+         (Quant q z (Alt.subst x t (Alt.subst v (Var z) f))).
+Proof.
+ intros.
+ rewrite subst_alt.
+ rewrite subst_QuGen with (z:=z); auto.
+ apply AEqQu_nosubst.
+ now rewrite !subst_alt.
+Qed.
+
+(*
+Lemma AlphaEq_equiv f f' : Alt.AlphaEq f f' <-> AlphaEq f f'.
+Proof.
+ rewrite <-nam2mix_canonical'. (* Vieille preuve!
+                                   nam2mix_canonical. *)
+Qed.
+
+Lemma AlphaEq_alt f f' :
+  Form.Alt.AlphaEq f f' <-> Form.AlphaEq f f'.
+Proof.
+ now rewrite AlphaEq_equiv, Alpha.AlphaEq_equiv.
+Qed.
+
+Lemma αeq_alt f f' : Alt.αeq f f' = αeq f f'.
+Proof.
+ apply eq_true_iff_eq. apply AlphaEq_alt.
+Qed.
+*)
