Equiv.v
@@ -1,16 +1,18 @@
 
-(** * Conversion from Named formulas to Locally Nameless formulas *)
+(** * Conversion between Named formulas and Locally Nameless formulas *)
 
 (** The NatDed development, Pierre Letouzey, 2019.
     This file is released under the CC0 License, see the LICENSE file *)
 
-Require Import Defs NameProofs Alpha.
-Require Nam Mix.
+Require Import Defs NameProofs Nam Alpha Subst Meta.
 Import ListNotations.
-Import Nam Nam.Form.
+Import Nam.Form.
 Local Open Scope bool_scope.
 Local Open Scope lazy_bool_scope.
 Local Open Scope eqb_scope.
+
+Implicit Types x y z v : variable.
+Implicit Types stack stk : list variable.
 
 (** From named to locally nameless *)
 
@@ -21,8 +23,7 @@ Fixpoint nam2mix_term stack t :=
     | None => Mix.FVar v
     | Some n => Mix.BVar n
     end
-  | Fun f args =>
-    Mix.Fun f (List.map (nam2mix_term stack) args)
+  | Fun f args => Mix.Fun f (List.map (nam2mix_term stack) args)
   end.
 
 Fixpoint nam2mix stack f :=
@@ -56,446 +57,565 @@ Fixpoint mix2nam stack f :=
     Nam.Quant q v (mix2nam (v::stack) f)
   end.
 
-(** Simultaneous renamings of many variables.
-    The bindings of this substitution will be handled in parallel,
-    not sequentially. In particular, the variables introduced
-    by a binding aren't modified by other bindings.
-    If the substitution contains several bindings of the same
-    variable, the leftmost binding wins (cf. [list_assoc]). *)
+(** Basic properties of [nam2mix] : level, free variables, etc *)
 
-Definition substitution := list (variable * term).
-
-Module Ren.
-
-Definition t := list (variable * variable).
-
-Definition invars (ren : t) :=
-  List.fold_right (fun p vs => Names.add (fst p) vs) Names.empty ren.
-
-Definition outvars (ren : t) :=
-  List.fold_right (fun p vs => Names.add (snd p) vs) Names.empty ren.
-
-Definition vars (ren : t) :=
-  Names.union (invars ren) (outvars ren).
-
-End Ren.
-
-(** First, we prove that [nam2mix] is canonical :
-    it sends alpha-equivalent named formulas to equal mixed formulas. *)
-
-(** The invariant used during the proof *)
-
-Module Nam2Mix.
-
-Inductive Inv (vars:Names.t) : Ren.t -> Ren.t -> Prop :=
- | InvNil : Inv vars [] []
- | InvCons v v' z sub sub' :
-   Inv vars sub sub' ->
-   ~Names.In z vars ->
-   ~Names.In z (Ren.vars sub) ->
-   ~Names.In z (Ren.vars sub') ->
-   Inv vars ((v,z)::sub) ((v',z)::sub').
-
-Inductive HalfInv (vars:Names.t) : Ren.t -> Prop :=
- | HInvNil : HalfInv vars []
- | HInvCons v z sub :
-   HalfInv vars sub ->
-   ~Names.In z vars ->
-   ~Names.In z (Ren.vars sub) ->
-   HalfInv vars ((v,z)::sub).
-
-End Nam2Mix.
-Import Nam2Mix.
-
-Hint Constructors Inv HalfInv.
-
-Lemma Inv_HalfInv vars sub sub' : Inv vars sub sub' -> HalfInv vars sub.
+Lemma nam2mix_term_level stack t :
+  Mix.level (nam2mix_term stack t) <= List.length stack.
 Proof.
- induction 1; auto.
+ revert t.
+ fix IH 1. destruct t; cbn.
+ - destruct (list_index v stack) eqn:E; cbn; auto with arith.
+   apply list_index_lt_length in E. omega.
+ - clear f. revert l.
+   fix IH' 1. destruct l as [|t l]; cbn; auto with arith.
+   apply Nat.max_lub; auto.
 Qed.
 
-Lemma Inv_HalfInv' vars sub sub' : Inv vars sub sub' -> HalfInv vars sub'.
+Lemma nam2mix_level stack f :
+  Mix.level (nam2mix stack f) <= List.length stack.
 Proof.
- induction 1; auto.
+ revert stack.
+ induction f; intros stack; cbn; auto with arith.
+ - apply (nam2mix_term_level stack (Nam.Fun "" l)).
+ - apply Nat.max_lub; auto.
+ - specialize (IHf (v::stack)). cbn in *. omega.
 Qed.
 
-Lemma Inv_sym vars sub sub' :
- Inv vars sub sub' -> Inv vars sub' sub.
+Lemma nam2mix_term_bclosed t :
+ Mix.BClosed (nam2mix_term [] t).
 Proof.
- induction 1; auto.
+ unfold Mix.BClosed.
+ generalize (nam2mix_term_level [] t); simpl; omega.
 Qed.
 
-Lemma Inv_notIn sub sub' vars v :
- Inv vars sub sub' ->
-  ~(Names.In v vars /\ Names.In v (Ren.outvars sub)).
+Lemma nam2mix_bclosed f :
+  Mix.BClosed (nam2mix [] f).
 Proof.
- induction 1; unfold Ren.vars in *; simpl; namedec.
+ unfold Mix.BClosed.
+ generalize (nam2mix_level [] f). simpl. auto with *.
 Qed.
 
-Lemma Inv_weak sub sub' vars vars' :
-  Names.Subset vars' vars -> Inv vars sub sub' -> Inv vars' sub sub'.
+Lemma nam2mix_tvars stk t :
+  Names.Equal (Mix.fvars (nam2mix_term stk t))
+              (Names.diff (Term.vars t) (Names.of_list stk)).
 Proof.
- induction 2; auto.
+ revert t.
+ fix IH 1. destruct t as [v|f l]; cbn.
+ - destruct list_index eqn:E; cbn.
+   + assert (NE : list_index v stk <> None) by congruence.
+     rewrite list_index_in in NE. rewrite <-names_of_list_in in NE. namedec.
+   + rewrite list_index_notin, <-names_of_list_in in E. namedec.
+ - clear f. revert l.
+   fix IH' 1. destruct l as [|t l]; cbn; rewrite ?IH, ?IH'; namedec.
 Qed.
 
-Lemma HalfInv_weak sub vars vars' :
-  Names.Subset vars' vars -> HalfInv vars sub -> HalfInv vars' sub.
+Lemma nam2mix_fvars stk f :
+  Names.Equal (Mix.fvars (nam2mix stk f))
+              (Names.diff (freevars f) (Names.of_list stk)).
 Proof.
- induction 2; auto.
-Qed.
-
-Lemma HalfInv_weak' (z:variable) sub vars vars' :
-  Names.Subset vars' (Names.add z vars) ->
-  ~Names.In z (Ren.vars sub) ->
-  HalfInv vars sub -> HalfInv vars' sub.
-Proof.
- induction 3; auto.
- constructor; auto.
- - apply IHHalfInv. unfold Ren.vars in *. simpl in H0. namedec.
- - rewrite H. unfold Ren.vars in *. simpl in *. namedec.
-Qed.
-
-Lemma list_assoc_some_in v sub z :
-  list_assoc v sub = Some z -> Names.In z (Ren.outvars sub).
-Proof.
- induction sub as [|(v',t) sub IH]; try easy.
- simpl.
- case eqbspec.
- - intros <- [= ->]. simpl. namedec.
- - intros _ E. apply IH in E. simpl. namedec.
-Qed.
-
-Lemma list_assoc_index vars v v' sub sub' z :
-Inv vars sub sub' ->
-list_assoc v sub = Some z ->
-list_assoc v' sub' = Some z ->
-exists k,
-list_index v (map fst sub) = Some k /\
-list_index v' (map fst sub') = Some k.
-Proof.
- induction 1; try easy.
- simpl.
- do 2 case eqbspec.
- - intros. now exists 0.
- - intros NE <- [= <-] E. apply list_assoc_some_in in E.
-   unfold Ren.vars in *. namedec.
- - intros <- NE E [= <-]. apply list_assoc_some_in in E.
-   unfold Ren.vars in *. namedec.
- - intros _ _ E E'. destruct (IHInv E E') as (k & Hk & Hk').
-   exists (S k). simpl in *. now rewrite Hk, Hk'.
-Qed.
-
-Lemma list_index_assoc vars v v' sub sub' n :
-Inv vars sub sub' ->
-list_index v (map fst sub) = Some n ->
-list_index v' (map fst sub') = Some n ->
-exists z,
-list_assoc v sub = Some z /\
-list_assoc v' sub' = Some z.
-Proof.
- intros inv.
- revert n.
- induction inv; try easy.
- simpl.
- do 2 case eqbspec.
- - intros <- <- n [= <-] _. now exists z.
- - intros _ <- n [= <-]. clear IHinv.
-   destruct list_index; simpl; congruence.
- - intros <- _ n E [= <-]. clear IHinv.
-   destruct list_index; simpl in *; congruence.
- - intros _ _ [|n].
-   destruct list_index; simpl; congruence.
-   intros E E'.
-   apply (IHinv n).
-   destruct (list_index v); simpl in *; congruence.
-   destruct (list_index v'); simpl in *; congruence.
-Qed.
-
-Fixpoint foldrename_term sub t :=
-  match sub with
-  | [] => t
-  | (v,z)::sub => foldrename_term sub (Term.subst v (Var z) t)
-  end.
-
-Fixpoint foldrename sub f :=
-  match sub with
-  | [] => f
-  | (v,z)::sub => foldrename sub (rename v z f)
-  end.
-
-Lemma foldrename_True sub : foldrename sub True = True.
-Proof.
- induction sub as [|(v,z) sub IH]; simpl; auto.
-Qed.
-
-Lemma foldrename_False sub : foldrename sub False = False.
-Proof.
- induction sub as [|(v,z) sub IH]; simpl; auto.
-Qed.
-
-Lemma foldrename_not sub f :
- foldrename sub (~f) = (~ foldrename sub f)%form.
-Proof.
- revert f.
- induction sub as [|(v,z) sub IH]; simpl; auto.
-Qed.
-
-Lemma foldrename_op sub o f f' :
- foldrename sub (Op o f f') = Op o (foldrename sub f) (foldrename sub f').
-Proof.
- revert f f'.
- induction sub as [|(v,z) sub IH]; simpl; auto.
-Qed.
-
-Lemma foldrename_quant_weak sub q v f :
- exists f', foldrename sub (Quant q v f) = Quant q v f'.
-Proof.
- revert f.
- induction sub as [|(x,z) sub IH]; simpl; auto.
- intros f. now exists f.
-Qed.
-
-Lemma foldrename_pred sub p l :
- foldrename sub (Pred p l) = Pred p (List.map (foldrename_term sub) l).
-Proof.
- revert l.
- induction sub as [|(x,z) sub IH]; simpl; auto.
- - intros l. f_equal. symmetry. apply map_id_iff; auto.
- - intros l. rewrite IH. f_equal. rewrite map_map; auto.
-Qed.
-
-Lemma foldrename_quant_swap sub f q (v:variable) :
- HalfInv (Names.add v (allvars f)) sub ->
- AlphaEq (foldrename sub (Quant q v f))
-         (Quant q v (foldrename (list_unassoc v sub) f)).
-Proof.
- revert f.
- induction sub as [|(x,t) sub IH].
- - simpl. reflexivity.
- - simpl. intros f. inversion 1; subst.
-   case eqbspec; simpl; auto.
-   intros NE.
-   apply IH; auto.
-   eapply HalfInv_weak'; eauto. rewrite allvars_rename. namedec.
-Qed.
-
-Lemma foldrename_rename_swap sub f (v z:variable) :
- HalfInv (Names.add v (allvars f)) ((v,z)::sub) ->
- AlphaEq (foldrename sub (rename v z f))
-         (rename v z (foldrename (list_unassoc v sub) f)).
-Proof.
- revert f.
- induction sub as [|(x,y) sub IH].
- - simpl. reflexivity.
- - simpl. intros f. inversion 1; subst.
-   inversion H3; subst.
-   simpl in H.
-   case eqbspec; simpl.
-   + intros ->.
-     rewrite rename_bis; auto with set.
-     apply IH. constructor; auto.
-     unfold Ren.vars in *. simpl in *; namedec.
-   + intros NE.
-     assert (z <> x).
-     { unfold Ren.vars in *; simpl in *; namedec. }
-     rewrite rename_rename; auto with set.
-     apply IH.
-     apply HalfInv_weak' with y (Names.add v (allvars f)).
-     rewrite allvars_rename; simpl. namedec.
-     unfold Ren.vars in *. simpl in *. namedec.
-     constructor; auto.
-     unfold Ren.vars in *. simpl in *; namedec.
-Qed.
-
-Lemma allvars_foldrename sub f :
-  Names.Subset (allvars (foldrename sub f))
-               (Names.union (Ren.outvars sub) (allvars f)).
-Proof.
- revert f.
- induction sub as [|(x,t) sub IH]; simpl; intros.
+ revert stk.
+ induction f; intros; cbn.
  - namedec.
- - rewrite IH, allvars_rename. namedec.
+ - namedec.
+ - apply (nam2mix_tvars stk (Fun "" l)).
+ - auto.
+ - rewrite IHf1, IHf2; namedec.
+ - rewrite IHf. simpl. namedec.
 Qed.
 
-Lemma unassoc_subset sub v :
- Names.Subset (Ren.outvars (list_unassoc v sub))
-              (Ren.outvars sub).
+(** [nam2mix] and modifying the stack while keeping the result *)
+
+Lemma nam2mix_term_indep stk stk' t :
+ (forall v, Names.In v (Term.vars t) ->
+            list_index v stk = list_index v stk') ->
+ nam2mix_term stk t = nam2mix_term stk' t.
 Proof.
- induction sub as [|(x,y) sub IH]; simpl.
- - auto with set.
- - case eqbspec; simpl; auto with set.
+ induction t as [v|f l IH] using term_ind'; cbn; intros Ht.
+ - rewrite Ht; auto with set.
+ - f_equal. clear f. apply map_ext_iff. intros a Ha.
+   apply IH; auto. intros v Hv. apply Ht.
+   rewrite unionmap_in. now exists a.
 Qed.
 
-Lemma foldrename_term_fun sub f l :
-  foldrename_term sub (Fun f l) = Fun f (map (foldrename_term sub) l).
+Lemma nam2mix_indep stk stk' f :
+ (forall v, Names.In v (freevars f) ->
+            list_index v stk = list_index v stk') ->
+ nam2mix stk f = nam2mix stk' f.
 Proof.
- revert f l.
- induction sub as [|(x,t) sub IH]; cbn; intros.
- - f_equal. symmetry. apply map_id.
- - rewrite IH. f_equal. apply map_map.
+ revert stk stk'.
+ induction f; simpl; intros stk stk' EQ; f_equal; auto with set.
+ - injection (nam2mix_term_indep stk stk' (Fun "" l)); auto.
+ - apply IHf. intros v' Hv'; simpl.
+   case eqbspec; auto.
+   intros NE. f_equal. apply EQ. namedec.
 Qed.
 
-Lemma foldrename_term_var_id sub (v:variable) :
-  ~ Names.In v (Ren.vars sub) ->
-  foldrename_term sub (Var v) = Var v.
+Lemma nam2mix_term_nostack stk t :
+ (forall v, In v stk -> ~Names.In v (Term.vars t)) ->
+ nam2mix_term stk t = nam2mix_term [] t.
 Proof.
- revert v.
- induction sub as [|(x,t) sub IH]; cbn; intros; auto.
- case eqbspec; auto.
- - intros <-. namedec.
- - intros NI. apply IH. unfold Ren.vars. namedec.
+ intros H. apply nam2mix_term_indep.
+ intros v Hv. simpl. rewrite list_index_notin.
+ intros IN. apply (H v IN Hv).
 Qed.
 
-Lemma foldrename_term_var sub (v:variable) :
- HalfInv (Names.singleton v) sub ->
- foldrename_term sub (Var v) = Var (list_assoc_dft v sub v).
+Lemma nam2mix_shadowstack stk x f :
+ In x stk ->
+ nam2mix (stk++[x]) f = nam2mix stk f.
 Proof.
- revert v.
- induction sub as [|(x,t) sub IH]; cbn; intros; auto.
- inversion H; subst.
- case eqbspec; auto.
- intros <-. apply foldrename_term_var_id; auto.
+ intros H. apply nam2mix_indep.
+ intros v Hv. case (eqbspec v x).
+ - intros ->. now rewrite list_index_app_l.
+ - intros NE. rewrite list_index_app_l'; auto. simpl; intuition.
 Qed.
 
-Lemma nam2mix_term_ok sub sub' t t' :
- Inv (Names.union (Term.vars t) (Term.vars t')) sub sub' ->
- foldrename_term sub t = foldrename_term sub' t' <->
- nam2mix_term (List.map fst sub) t = nam2mix_term (List.map fst sub') t'.
+Lemma nam2mix_shadowstack' stk stk' x y f :
+ In x stk \/ ~Names.In x (freevars f) ->
+ In y stk \/ ~Names.In y (freevars f) ->
+ nam2mix (stk++x::stk') f = nam2mix (stk++y::stk') f.
 Proof.
- revert t t'.
- fix IH 1. destruct t as [|f l], t' as [|f' l']; cbn; intro IV.
- - rewrite !foldrename_term_var.
-   2:{ eapply Inv_HalfInv'; eauto. eapply Inv_weak; eauto. namedec. }
-   2:{ eapply Inv_HalfInv; eauto. eapply Inv_weak; eauto. namedec. }
-   rewrite !list_assoc_dft_alt.
-   split.
-   + destruct (list_assoc v sub) as [z|] eqn:EQ;
-     destruct (list_assoc v0 sub') as [z'|] eqn:EQ'.
-     * intros [= <-].
-       destruct (list_assoc_index _ v v0 _ _ z IV) as (n & -> & ->); auto.
-     * intros [=].
-       apply list_assoc_some_in in EQ.
-       apply (Inv_notIn _ _ _ z) in IV. namedec.
-     * intros [=].
-       apply list_assoc_some_in in EQ'.
-       apply Inv_sym in IV.
-       apply (Inv_notIn _ _ _ z') in IV. namedec.
-     * intros [= <-].
-       rewrite list_assoc_index_none in EQ. rewrite EQ.
-       rewrite list_assoc_index_none in EQ'. now rewrite EQ'.
-   + destruct (list_index v (map fst sub)) as [n|] eqn:EQ;
-     destruct (list_index v0 (map fst sub')) as [n'|] eqn:EQ'; try easy.
-     * injection 1 as <-.
-       destruct (list_index_assoc _ v v0 _ _ n IV) as (t & -> & ->); auto.
-     * injection 1 as <-.
-       rewrite <- list_assoc_index_none in EQ. rewrite EQ.
-       rewrite <- list_assoc_index_none in EQ'. now rewrite EQ'.
- - rewrite foldrename_term_fun.
-   rewrite foldrename_term_var.
-   2:{ eapply Inv_HalfInv; eauto. eapply Inv_weak; eauto. namedec. }
-   destruct list_index; easy.
- - rewrite foldrename_term_fun.
-   rewrite foldrename_term_var.
-   2:{ eapply Inv_HalfInv'; eauto. eapply Inv_weak; eauto. namedec. }
-   destruct list_index; easy.
- - rewrite !foldrename_term_fun.
-   assert
-     (map (foldrename_term sub) l = map (foldrename_term sub') l'
-      <-> map (nam2mix_term (map fst sub)) l =
-          map (nam2mix_term (map fst sub')) l').
-   { revert l l' IV.
-     fix IH' 1. destruct l as [|t l], l' as [|t' l']; cbn; intros IV;
-      try easy.
-     split.
-     - injection 1 as EQt EQl. f_equal.
-       + apply IH; auto. eapply Inv_weak; eauto. namedec.
-       + apply IH'; auto. eapply Inv_weak; eauto. namedec.
-     - injection 1 as EQt EQl. f_equal.
-       + apply IH; auto. eapply Inv_weak; eauto. namedec.
-       + apply IH'; auto. eapply Inv_weak; eauto. namedec. }
-   split; injection 1 as <- EQ; f_equal; intuition.
+ intros Hx Hy. apply nam2mix_indep.
+ intros v Hv.
+ destruct (in_dec string_dec v stk).
+ - rewrite 2 list_index_app_l; auto.
+ - rewrite 2 list_index_app_r; auto. simpl.
+   case eqbspec; [intros ->;intuition|].
+   case eqbspec; [intros ->;intuition|auto].
+Qed.
+
+(** [nam2mix] and [partialsubst] *)
+
+Lemma nam2mix_term_subst stk x u t:
+ ~In x stk ->
+ nam2mix_term stk (Term.subst x u t) =
+ Mix.fsubst x (nam2mix_term stk u) (nam2mix_term stk t).
+Proof.
+ induction t as [v|f l IH] using term_ind'; intros NI; cbn.
+ - case eqbspec.
+   + intros ->.
+     rewrite <-list_index_notin in NI. rewrite NI.
+     cbn. unfold Mix.varsubst. now rewrite eqb_refl.
+   + intros NE.
+     cbn.
+     destruct (list_index v stk); cbn; auto.
+     unfold Mix.varsubst. case eqbspec; congruence.
+ - f_equal; clear f.
+   rewrite !map_map.
+   apply map_ext_in. intros t Ht. apply IH; auto.
+Qed.
+
+Lemma nam2mix_partialsubst stk x u f :
+ ~In x stk ->
+ (forall v, In v stk -> ~Names.In v (Term.vars u)) ->
+ IsSimple x u f ->
+ nam2mix stk (partialsubst x u f) =
+ Mix.fsubst x (nam2mix_term [] u) (nam2mix stk f).
+Proof.
+ revert stk.
+ induction f; cbn; intros stk Hx Hu IS; f_equal; auto.
+ - rewrite <- (nam2mix_term_nostack stk); auto.
+   injection (nam2mix_term_subst stk x u (Fun "" l)); easy.
+ - intuition.
+ - intuition.
+ - case eqbspec; cbn.
+   + intros ->.
+     unfold Mix.fsubst.
+     rewrite form_vmap_id; auto.
+     intros x. rewrite nam2mix_fvars. simpl.
+     unfold Mix.varsubst.
+     intros IN.
+     case eqbspec; auto. intros <-. namedec.
+   + intros NE.
+     destruct IS as [-> | (NI,IS)]; [easy|].
+     apply IHf; simpl; intuition; subst; eauto.
+Qed.
+
+Lemma nam2mix_term_subst' stk stk' x z t :
+ ~In x stk ->
+ ~In z stk ->
+ ~Names.In z (Term.vars t) ->
+ nam2mix_term (stk++z::stk') (Term.subst x (Var z) t) =
+ nam2mix_term (stk++x::stk') t.
+Proof.
+ induction t as [v|f l IH] using term_ind'; intros Hx Hz NI; cbn in *.
+ - case eqbspec; cbn.
+   + intros ->.
+     rewrite 2 list_index_app_r by intuition.
+     simpl; rewrite 2 eqb_refl. simpl; auto.
+   + intros NE. destruct (In_dec string_dec v stk).
+     * rewrite 2 list_index_app_l; auto.
+     * rewrite 2 list_index_app_r by auto. simpl.
+       do 2 case eqbspec; auto. namedec. intuition.
+ - f_equal; clear f.
+   rewrite !map_map.
+   apply map_ext_in. intros t Ht. apply IH; auto.
+   eapply unionmap_notin; eauto.
+Qed.
+
+Lemma nam2mix0_partialsubst x u f :
+ IsSimple x u f ->
+ nam2mix [] (partialsubst x u f) =
+  Mix.fsubst x (nam2mix_term [] u) (nam2mix [] f).
+Proof.
+ apply nam2mix_partialsubst; auto.
+Qed.
+
+Lemma nam2mix_rename stk stk' x z f :
+ ~In x stk ->
+ ~In z stk ->
+ ~Names.In z (allvars f) ->
+ nam2mix (stk++z::stk') (rename x z f) =
+ nam2mix (stk++x::stk') f.
+Proof.
+ revert stk.
+ induction f; cbn; intros stk Hx Hz IS; f_equal; auto.
+ - injection (nam2mix_term_subst' stk stk' x z (Fun "" l)); easy.
+ - intuition.
+ - intuition.
+ - case eqbspec; cbn.
+   + intros <-.
+     symmetry.
+     apply (nam2mix_shadowstack' (x::stk)). simpl; auto.
+     right. rewrite freevars_allvars. namedec.
+   + intros NE.
+     apply (IHf (v::stk)).
+     simpl. intuition.
+     simpl. intuition.
+     namedec.
+Qed.
+
+Lemma term_subst_bsubst stk x u t :
+ ~In x stk ->
+ (forall v, In v stk -> ~Names.In v (Term.vars u)) ->
+ nam2mix_term stk (Term.subst x u t) =
+  Mix.bsubst (length stk) (nam2mix_term [] u)
+             (nam2mix_term (stk++[x]) t).
+Proof.
+  induction t as [v|f l IH] using term_ind'; intros X U; cbn in *.
+ - case eqbspec.
+   + intros ->.
+     rewrite list_index_app_r; auto. cbn. rewrite eqb_refl. cbn.
+     rewrite Nat.add_0_r. rewrite eqb_refl.
+     now apply nam2mix_term_nostack.
+   + intros NE. cbn.
+     rewrite list_index_app_l' by (simpl; intuition).
+     destruct (list_index v stk) eqn:E; cbn; auto.
+     apply list_index_lt_length in E.
+     case eqbspec; intros; subst; auto; omega.
+ - f_equal; clear f.
+   rewrite !map_map.
+   apply map_ext_in. intros t Ht. apply IH; auto.
+Qed.
+
+Lemma partialsubst_bsubst stk x u f :
+ ~In x stk ->
+ (forall v, In v stk -> ~Names.In v (Term.vars u)) ->
+ IsSimple x u f ->
+ nam2mix stk (partialsubst x u f) =
+  Mix.bsubst (length stk) (nam2mix_term [] u)
+             (nam2mix (stk++[x]) f).
+Proof.
+ revert stk.
+ induction f; cbn; intros stk X U IS; f_equal; auto.
+ - injection (term_subst_bsubst stk x u (Fun "" l)); auto.
+ - destruct IS as (IS1,IS2); auto.
+ - destruct IS as (IS1,IS2); auto.
+ - case eqbspec; cbn.
+   + intros <-.
+     change (x::stk++[x]) with ((x::stk)++[x]).
+     rewrite nam2mix_shadowstack by (simpl; auto).
+     symmetry.
+     apply form_level_bsubst_id.
+     now rewrite nam2mix_level.
+   + intros NE.
+     destruct IS as [->|(NI,IS)]; [easy|].
+     apply IHf; simpl; auto.
+     intuition.
+     intros y [<-|Hy]; auto.
+Qed.
+
+Lemma partialsubst_bsubst0 x u f :
+ IsSimple x u f ->
+ nam2mix [] (partialsubst x u f) =
+  Mix.bsubst 0 (nam2mix_term [] u) (nam2mix [x] f).
+Proof.
+ apply partialsubst_bsubst; auto.
+Qed.
+
+Lemma rename_bsubst0 x z f :
+ ~Names.In z (allvars f) ->
+ nam2mix [] (rename x z f) =
+  Mix.bsubst 0 (Mix.FVar z) (nam2mix [x] f).
+Proof.
+ intros.
+ rewrite rename_partialsubst by auto.
+ apply (partialsubst_bsubst0 x (Var z)); auto.
+Qed.
+
+Lemma nam2mix_rename_iff z v v' f f' :
+  ~ Names.In z (Names.union (allvars f) (allvars f')) ->
+  nam2mix [] (rename v z f) = nam2mix [] (rename v' z f')
+  <->
+  nam2mix [v] f = nam2mix [v'] f'.
+Proof.
+ intros Hz.
+ rewrite 2 rename_bsubst0 by namedec.
+ split.
+ - intros H. apply bsubst_fresh_inj in H; auto.
+   rewrite !nam2mix_fvars. cbn. rewrite !freevars_allvars. namedec.
+ - now intros ->.
 Qed.
 
 Lemma nam2mix_term_inj t t' :
  nam2mix_term [] t = nam2mix_term [] t' <-> t = t'.
 Proof.
- split; [|now intros ->].
- rewrite <- (nam2mix_term_ok [] []); auto.
+ split; [ | intros <-; auto ].
+ revert t t'.
+ fix IH 1. destruct t, t'; cbn; try easy.
+ - now intros [= <-].
+ - intros [= <- EQ]. f_equal.
+   revert l l0 EQ.
+   fix IH' 1. destruct l, l0; cbn; try easy.
+   intros [= EQ EQ']. f_equal; auto.
 Qed.
 
-Lemma nam2mix_canonical_gen sub sub' f f' :
- Inv (Names.union (allvars f) (allvars f')) sub sub' ->
- AlphaEq (foldrename sub f) (foldrename sub' f') <->
- nam2mix (List.map fst sub) f = nam2mix (List.map fst sub') f'.
-Proof.
- revert f' sub sub'.
- induction f; destruct f'; intros sub sub'; simpl; intros IV;
-  rewrite ?foldrename_True, ?foldrename_False, ?foldrename_not, ?foldrename_op,
-    ?foldrename_pred; try easy;
-  try (destruct (foldrename_quant_weak sub q v f) as (g,->); easy);
-  try (destruct (foldrename_quant_weak sub' q v f') as (g',->); easy).
- - destruct (nam2mix_term_ok sub sub' (Fun "" l) (Fun "" l0) IV) as (U,V).
-   rewrite !foldrename_term_fun in *. cbn in *.
-   split.
-   + inversion 1; subst. f_equal. injection U; auto. now f_equal.
-   + injection 1 as <- EQ. injection V; auto. now intros ->. now f_equal.
- - split.
-   + inversion_clear 1. f_equal. apply IHf; auto.
-   + injection 1. rewrite <- IHf; auto.
- - split.
-   + inversion_clear 1. f_equal.
-     * apply IHf1; auto. eapply Inv_weak; eauto. namedec.
-     * apply IHf2; auto. eapply Inv_weak; eauto. namedec.
-   + injection 1 as <- EQ1 EQ2.
-     rewrite <- IHf1 in EQ1 by (eapply Inv_weak; eauto; namedec).
-     rewrite <- IHf2 in EQ2 by (eapply Inv_weak; eauto; namedec).
-     auto.
- - destruct (exist_fresh
-               (Names.union
-                  (Names.union (Ren.vars sub) (Ren.vars sub'))
-                  (Names.union (Names.add v (allvars f))
-                               (Names.add v0 (allvars f'))))) as (z,Hz).
-   assert (HalfInv (Names.add v (allvars f)) sub).
-   { eapply Inv_HalfInv; eauto. eapply Inv_weak; eauto. namedec. }
-   assert (HalfInv (Names.add v0 (allvars f')) sub').
-   { eapply Inv_HalfInv'; eauto. eapply Inv_weak; eauto. namedec. }
-   split.
-   + intros EQ.
-     assert (q = q0).
-     { destruct (foldrename_quant_weak sub q v f) as (g,->) in EQ.
-       destruct (foldrename_quant_weak sub' q0 v0 f') as (g',->) in EQ.
-       inversion_clear EQ; auto. }
-     subst q0. f_equal.
-     change (nam2mix (map fst ((v,z)::sub)) f =
-             nam2mix (map fst ((v0,z)::sub')) f').
-     apply IHf.
-     { constructor; auto with set.
-       eapply Inv_weak; eauto. namedec. }
-     { simpl.
-       rewrite !foldrename_rename_swap by (constructor; auto with set).
-       rewrite !foldrename_quant_swap in EQ; auto.
-       apply AEqQu_iff with q; auto.
-       rewrite !allvars_foldrename.
-       rewrite !unassoc_subset. unfold Ren.vars in Hz. namedec. }
-   + injection 1 as <- EQ.
-     change (nam2mix (map fst ((v,z)::sub)) f =
-             nam2mix (map fst ((v0,z)::sub')) f') in EQ.
-     rewrite <- IHf in EQ.
-     2:{ constructor; auto with set.
-         eapply Inv_weak; eauto. namedec. }
-     simpl in EQ.
-     rewrite !foldrename_rename_swap in EQ by (constructor; auto with set).
-     rewrite !foldrename_quant_swap; auto.
-     eapply AEqQu; eauto.
-     rewrite !allvars_foldrename.
-     rewrite !unassoc_subset. unfold Ren.vars in Hz. namedec.
-Qed.
-
-Lemma nam2mix_canonical (f f' : Nam.formula) :
+Lemma nam2mix_canonical f f' :
  nam2mix [] f = nam2mix [] f' <-> AlphaEq f f'.
 Proof.
- symmetry.
- apply (nam2mix_canonical_gen [] []). constructor.
+ split.
+ - set (h := S (Nat.max (height f) (height f'))).
+   assert (LT : height f < h) by (unfold h; auto with *).
+   assert (LT' : height f' < h) by (unfold h; auto with *).
+   clearbody h. revert f f' LT LT'.
+   induction h as [|h IH]; [inversion 1|].
+   destruct f, f'; simpl; intros LT LT'; simpl_height; try easy.
+   + intros [= <- E].
+     destruct (nam2mix_term_inj (Fun "" l) (Fun "" l0)) as (H,_).
+     simpl in H. injection H as <-; auto. now f_equal.
+   + intros [= E]; auto.
+   + intros [= <- E1 E2]; auto.
+   + intros [= <- E].
+     destruct (exist_fresh (Names.union (allvars f) (allvars f'))) as (z,Hz).
+     apply AEqQu with z; auto.
+     apply IH; try rewrite rename_height; auto.
+     apply nam2mix_rename_iff; auto.
+ - induction 1; cbn; f_equal; auto.
+   apply (nam2mix_rename_iff z); auto.
+Qed.
+
+(** We've just seen that [nam2mix []] maps alpha-equivalent formulas
+    to equal formulas. This is actually also true for
+    [nam2mix stk] with any [stk]. Here comes a first part
+    of this statement, the full version is below in
+    [nam2mix_canonical_gen].
+*)
+
+Lemma AlphaEq_nam2mix_gen stk f f' :
+ AlphaEq f f' -> nam2mix stk f = nam2mix stk f'.
+Proof.
+ intros H. revert stk.
+ induction H; cbn; intros stk; f_equal; auto.
+ generalize (IHAlphaEq (z::stk)).
+ rewrite (nam2mix_rename [] stk v z) by (auto; namedec).
+ rewrite (nam2mix_rename [] stk v' z) by (auto; namedec).
+ auto.
+Qed.
+
+(** SUBST *)
+
+Lemma nam2mix_Subst_fsubst stk x u f f' :
+ ~In x stk ->
+ (forall v, In v stk -> ~Names.In v (Term.vars u)) ->
+ Subst x u f f' ->
+ nam2mix stk f' = Mix.fsubst x (nam2mix_term [] u) (nam2mix stk f).
+Proof.
+ intros NI CL (f0 & EQ & SI).
+ apply AlphaEq_nam2mix_gen with (stk:=stk) in EQ. rewrite EQ.
+ apply SimpleSubst_carac in SI. destruct SI as (<- & IS).
+ apply nam2mix_partialsubst; auto.
+Qed.
+
+Lemma nam2mix_subst_fsubst stk x u f :
+ ~In x stk ->
+ (forall v, In v stk -> ~Names.In v (Term.vars u)) ->
+ nam2mix stk (subst x u f) =
+ Mix.fsubst x (nam2mix_term [] u) (nam2mix stk f).
+Proof.
+ intros.
+ apply nam2mix_Subst_fsubst; auto.
+ apply Subst_subst.
+Qed.
+
+Lemma nam2mix0_subst_fsubst x u f :
+ nam2mix [] (subst x u f) =
+  Mix.fsubst x (nam2mix_term [] u) (nam2mix [] f).
+Proof.
+ apply nam2mix_subst_fsubst; auto.
+Qed.
+
+Lemma nam2mix_Subst_bsubst stk x u f f' :
+ ~In x stk ->
+ (forall v, In v stk -> ~Names.In v (Term.vars u)) ->
+ Subst x u f f' ->
+ nam2mix stk f' =
+ Mix.bsubst (length stk) (nam2mix_term [] u)
+            (nam2mix (stk++[x]) f).
+Proof.
+ intros NI CL (f0 & EQ & SI).
+ apply AlphaEq_nam2mix_gen with (stk:=stk++[x]) in EQ.
+ rewrite EQ.
+ apply SimpleSubst_carac in SI. destruct SI as (<- & IS).
+ now apply partialsubst_bsubst.
+Qed.
+
+Lemma nam2mix_subst_bsubst stk x u f :
+ ~In x stk ->
+ (forall v, In v stk -> ~Names.In v (Term.vars u)) ->
+ nam2mix stk (subst x u f) =
+  Mix.bsubst (length stk) (nam2mix_term [] u)
+             (nam2mix (stk++[x]) f).
+Proof.
+ intros.
+ apply nam2mix_Subst_bsubst; auto.
+ apply Subst_subst.
+Qed.
+
+Lemma nam2mix_subst_bsubst0 x u f :
+ nam2mix [] (subst x u f) =
+  Mix.bsubst 0 (nam2mix_term [] u) (nam2mix [x] f).
+Proof.
+ apply nam2mix_subst_bsubst; auto.
+Qed.
+
+Lemma nam2mix_rename_iff2 z v v' f f' :
+  ~ Names.In z (Names.union (freevars f) (freevars f')) ->
+  nam2mix [] (subst v (Var z) f) =
+  nam2mix [] (subst v' (Var z) f')
+  <->
+  nam2mix [v] f = nam2mix [v'] f'.
+Proof.
+ intros Hz.
+ rewrite 2 nam2mix_subst_bsubst0. cbn.
+ split.
+ - intros H. apply bsubst_fresh_inj in H; auto.
+   rewrite !nam2mix_fvars. cbn. namedec.
+ - now intros ->.
+Qed.
+
+Lemma nam2mix_subst_nop x f :
+  nam2mix [] (subst x (Var x) f) = nam2mix [] f.
+Proof.
+ rewrite nam2mix0_subst_fsubst. simpl.
+ unfold Mix.fsubst.
+ apply form_vmap_id.
+ intros y Hy. unfold Mix.varsubst.
+ case eqbspec; intros; subst; auto.
+Qed.
+
+Lemma subst_nop x f :
+  AlphaEq (subst x (Var x) f) f.
+Proof.
+ apply nam2mix_canonical.
+ apply nam2mix_subst_nop.
+Qed.
+
+Lemma nam2mix_rename_iff3 v x f f' :
+  ~ Names.In x (Names.remove v (freevars f)) ->
+  nam2mix [] (subst v (Var x) f) = nam2mix [] f'
+  <->
+  nam2mix [v] f = nam2mix [x] f'.
+Proof.
+ intros Hx.
+ rewrite nam2mix_subst_bsubst0. cbn.
+ split.
+ - rewrite <- (nam2mix_subst_nop x f').
+   rewrite nam2mix_subst_bsubst0. cbn.
+   apply bsubst_fresh_inj.
+   rewrite !nam2mix_fvars. cbn. namedec.
+ - intros ->.
+   rewrite <- (nam2mix_subst_bsubst0 x (Var x)).
+   apply nam2mix_subst_nop.
+Qed.
+
+Lemma nam2mix_nostack stk f f' :
+ nam2mix stk f = nam2mix stk f' <->
+ nam2mix [] f = nam2mix [] f'.
+Proof.
+ split.
+ - rewrite <- (rev_involutive stk).
+   set (s := rev stk). clearbody s.
+   revert f f'.
+   induction s as [|x s IH].
+   + trivial.
+   + intros f f'. simpl.
+     destruct (List.In_dec string_dec x (rev s)) as [IN|NI].
+     * rewrite 2 nam2mix_shadowstack; auto.
+     * intros Eq.
+       apply IH.
+       assert (E := subst_nop x f).
+       apply AlphaEq_nam2mix_gen with (stk:=rev s) in E.
+       rewrite <- E.
+       assert (E' := subst_nop x f').
+       apply AlphaEq_nam2mix_gen with (stk:=rev s) in E'.
+       rewrite <- E'.
+       clear E E'.
+       rewrite !nam2mix_subst_bsubst, Eq; simpl; auto.
+       intros v Hv. nameiff. now intros ->.
+       intros v Hv. nameiff. now intros ->.
+ - rewrite nam2mix_canonical. apply AlphaEq_nam2mix_gen.
+Qed.
+
+(** TODO Again !! *)
+
+Lemma nam2mix_canonical_gen stk f f' :
+ nam2mix stk f = nam2mix stk f' <-> AlphaEq f f'.
+Proof.
+ rewrite nam2mix_nostack. apply nam2mix_canonical.
+Qed.
+
+(** Swapping substitutions.
+    This technical lemma is described in Alexandre's course notes.
+    See also [Alpha.partialsubst_partialsubst]. In fact, we won't
+    reuse it afterwards. *)
+
+Lemma subst_subst x x' u u' f :
+ x<>x' -> ~Names.In x (Term.vars u') ->
+ AlphaEq (subst x' u' (subst x u f))
+         (subst x (Term.subst x' u' u) (subst x' u' f)).
+Proof.
+ intros NE NI.
+ apply nam2mix_canonical.
+ rewrite !nam2mix0_subst_fsubst.
+ rewrite nam2mix_term_subst by auto.
+ apply form_fsubst_fsubst; auto.
+ rewrite nam2mix_tvars. cbn. namedec.
+Qed.
+
+(** The general equation defining [subst] on a quantified formula,
+    via renaming. *)
+
+Lemma subst_QuGen x z t q v f :
+ x<>v ->
+ ~Names.In z (Names.add x (Names.union (freevars f) (Term.vars t))) ->
+ AlphaEq (subst x t (Quant q v f))
+         (Quant q z (subst x t (subst v (Var z) f))).
+Proof.
+ intros NE NI.
+ apply nam2mix_canonical. cbn - [subst].
+ rewrite !nam2mix0_subst_fsubst. cbn - [subst].
+ f_equal.
+ rewrite nam2mix_subst_fsubst by (simpl; namedec).
+ f_equal.
+ apply nam2mix_rename_iff3; auto. namedec.
+Qed.
+
+Lemma nam2mix_eqb (f f' : Nam.formula) :
+ (nam2mix [] f =? nam2mix [] f') = (f =? f').
+Proof.
+ case eqbspec; rewrite nam2mix_canonical.
+ - intros. symmetry. now apply AlphaEq_equiv.
+ - intros H. rewrite <- AlphaEq_equiv in H.
+   symmetry. exact (not_true_is_false _ H).
 Qed.
 
 (** Proofs about [mix2nam] *)
@@ -570,42 +690,6 @@ Proof.
  simpl. rewrite E. auto.
 Qed.
 
-Lemma nam2mix_term_level stack t :
-  Mix.level (nam2mix_term stack t) <= List.length stack.
-Proof.
- revert t.
- fix IH 1. destruct t; cbn.
- - destruct (list_index v stack) eqn:E; cbn; auto with arith.
-   apply list_index_lt_length in E. omega.
- - clear f. revert l.
-   fix IH' 1. destruct l as [|t l]; cbn; auto with arith.
-   apply Nat.max_lub; auto.
-Qed.
-
-Lemma nam2mix_level stack f :
-  Mix.level (nam2mix stack f) <= List.length stack.
-Proof.
- revert stack.
- induction f; intros stack; cbn; auto with arith.
- - apply (nam2mix_term_level stack (Nam.Fun "" l)).
- - apply Nat.max_lub; auto.
- - specialize (IHf (v::stack)). cbn in *. omega.
-Qed.
-
-Lemma nam2mix_term_bclosed t :
- Mix.BClosed (nam2mix_term [] t).
-Proof.
- unfold Mix.BClosed.
- generalize (nam2mix_term_level [] t); simpl; omega.
-Qed.
-
-Lemma nam2mix_bclosed f :
-  Mix.BClosed (nam2mix [] f).
-Proof.
- unfold Mix.BClosed.
- generalize (nam2mix_level [] f). simpl. auto with *.
-Qed.
-
 Lemma nam_mix_nam_term t :
  mix2nam_term [] (nam2mix_term [] t) = t.
 Proof.
@@ -620,13 +704,4 @@ Proof.
  apply nam2mix_canonical.
  apply mix_nam_mix.
  apply nam2mix_bclosed.
-Qed.
-
-Lemma nam2mix_eqb (f f' : Nam.formula) :
- (nam2mix [] f =? nam2mix [] f') = (f =? f').
-Proof.
- case eqbspec; rewrite nam2mix_canonical.
- - intros. symmetry. now apply AlphaEq_equiv.
- - intros H. rewrite <- AlphaEq_equiv in H.
-   symmetry. exact (not_true_is_false _ H).
 Qed.
